EffectSSA/Semantics/Lemmas.lean
@@ -1,0 +1,18 @@
+import EffectSSA.Syntax
+import EffectSSA.Semantics.Program
+
+/-!
+# Lemmas about semantics
+-/
+namespace EffectSSA
+variable {τ} [MemoryModel τ]
+
+/-
+The following theorem does not quite work, because the `.results` are not
+nicely def-eq.
+-/
+-- theorem Program.exec_append (p : Program τ n) (q : Program τ p.results) :
+--     (p.append q).exec =
+--       have h := sorry
+--       fun env => (p.exec env >>= (q.cast h).exec) := by
+--   sorry
