EffectSSA/Syntax.lean
@@ -2,3 +2,4 @@ import EffectSSA.Syntax.Basic
 import EffectSSA.Syntax.Var
 import EffectSSA.Syntax.Repr
 import EffectSSA.Syntax.Notation
+import EffectSSA.Syntax.Lemmas
