EffectSSA/Syntax/Lemmas.lean
@@ -1,0 +1,61 @@
+import EffectSSA.Syntax.Basic
+
+/-!
+# Syntax lemmas
+-/
+namespace EffectSSA
+variable {τ : Ty} -- [MemorySignature τ]
+
+/-!
+## Casting
+--------------------------------------------------------------------------------
+-/
+
+/--
+Change the bound of an instruction to a provably equal bound.
+-/
+def Instruction.cast (h : n = m) : Instruction τ n → Instruction τ m
+  -- TODO: generate this function
+  | _ => sorry
+
+@[simp]
+theorem Instruction.results_cast (h : n = m) (i : Instruction τ n) :
+    (i.cast h).results = i.results := by
+  sorry
+
+/--
+Change the bound of a program to a provably equal bound.
+-/
+def Program.cast (h : n = m) : Program τ n → Program τ m
+  | .nil => .nil
+  | i ;> p => (i.cast h) ;> (p.cast <| by simp)
+
+/-!
+## Program Lemmas
+--------------------------------------------------------------------------------
+-/
+namespace Program
+
+/-! ### `results` -/
+
+@[simp]
+theorem results_nil (n : Nat) :
+    (.nil : Program τ n).results = n := by
+  rfl
+
+@[simp]
+theorem results_cons {i : Instruction τ n} {p : Program τ i.results} :
+    (i ;> p).results = p.results := by
+  simp [results]
+
+@[simp]
+theorem results_append {p : Program τ n} {q : Program τ p.results} :
+    (p.append q).results = q.results := by
+  induction p <;> simp_all [append]
+
+@[simp]
+theorem results_cast (h : n = m) (p : Program τ n) :
+    (p.cast h).results = p.results := by
+  induction p generalizing m <;> simp_all [cast]
+
+end Program
